Defined the language of system F

formalizing/SystemF/lang.v
@@ -13,15 +13,19 @@ Delimit Scope val_scope with V.
 
 (** ** Expressions and Values *)
 Inductive base_lit : Set :=
-  | LitInt (n : Z) | LitBool (b : bool) | LitUnit.
+  | LitInt (n : Z) | LitBool (b : bool) | LitString (s : string) | LitUnit.
 Inductive un_op : Set :=
   | NegOp (* Boolean Negation *)
   | MinusUnOp (* Integer Negation *)
+  | LenOp (* String Length *)
   .
 Inductive bin_op : Set :=
-  | PlusOp | MinusOp | MultOp | DivOp | ModOp (* Integer Arithmetics *)
-  | LtOp | LeOp | EqOp (* Integer Comparisons *)
-  | AndOp | OrOp (* Logical Operators *)
+  | PlusOp | MinusOp | MultOp (* Integer Arithmetics *)
+  | LtOp | LeOp | GtOp | GeOp (* Integer Comparisons *)
+  | AndOp | OrOp | SubOp (* Logical Operators *)
+  | ConcatOp (* String Concatenation *)
+  | PrefixOp | SubstrOp (* String Prefix/Substring Relations *)
+  | EqOp | NeqOp (* Literal Comparisons *)
   .
 
 
@@ -62,6 +66,7 @@ Inductive val :=
 
 Bind Scope val_scope with val.
 
+(* Conversion from values to expressions *)
 Fixpoint of_val (v : val) : expr :=
   match v with
   | LitV l => Lit l
@@ -73,15 +78,360 @@ Fixpoint of_val (v : val) : expr :=
   | InjRV v => InjR (of_val v)
   end.
 
+(* Conversion from expressions to values *)
+(* Returns None if the expression is not a value *)
 Fixpoint to_val (e : expr) : option val :=
   match e with
   | Lit l => Some $ LitV l
   | Lam x e' => Some $ LamV x e'
   | TLam e' => Some $ TLamV e'
-  | Pack e' => to_val e' ≫= (λ v, Some $ PackV v)
+  | Pack e' => PackV <$> to_val e'
   | Pair e1 e2 =>
       to_val e1 ≫= (λ v1, to_val e2 ≫= (λ v2, Some $ PairV v1 v2))
-  | InjL e' => to_val e' ≫= (λ v, Some $ InjLV v)
-  | InjR e' => to_val e' ≫= (λ v, Some $ InjRV v)
+  | InjL e' => InjLV <$> to_val e'
+  | InjR e' => InjRV <$> to_val e'
   | _ => None
   end.
+
+(** ** Properties of Conversion Functions *)
+Lemma to_of_val v : to_val (of_val v) = Some v.
+Proof. by induction v; simplify_option_eq. Qed.
+
+Lemma of_to_val e v : to_val e = Some v → of_val v = e.
+Proof. revert v; induction e; intros; simplify_option_eq; auto with f_equal. Qed.
+
+#[export] Instance of_val_inj : Inj (=) (=) of_val.
+Proof. by intros ?? H; apply (inj Some); rewrite <-!to_of_val, H. Qed.
+
+
+(* Coq prop representing the given expression being a value *)
+Fixpoint is_val (e : expr) : Prop :=
+  match e with 
+  | Lit _ | Lam _ _ | TLam _ => True
+  | Pack e' | InjL e' | InjR e' => is_val e'
+  | Pair e1 e2 => is_val e1 ∧ is_val e2
+  | _ => False
+  end.
+
+Lemma is_val_spec e :
+  is_val e ↔ ∃ v, to_val e = Some v.
+Proof.
+  split; intro H.
+  - induction e; cycle 11; simpl; try by eauto.
+    2-4: apply IHe in H as [v ->]; eauto.
+    destruct H as [H1 H2].
+    apply IHe1 in H1 as [v1 ->]; apply IHe2 in H2 as [v2 ->]; eauto.
+  - destruct H as [v Hv]. rewrite <-(of_to_val e v); eauto.
+    induction v in e |-*; simpl; eauto.
+Qed.
+
+Ltac simplify_val :=
+  repeat match goal with
+  | H: context[to_val (of_val ?v)] |- _ =>
+      do !rewrite to_of_val in H
+  | H: is_val ?e |- _ =>
+      let v := fresh "v" in
+      let Hv := fresh "H" v in
+      destruct (proj1 (is_val_spec e) H) as [v Hv]; clear H
+  | H: to_val ?e = Some ?v |- _ =>
+      assert (e = of_val v) as -> by (apply of_to_val in H; auto); clear H
+  | |- context[to_val (of_val ?v)] =>
+      do !rewrite to_of_val
+  end.
+
+Tactic Notation "solve_val" "by" tactic(tac) :=
+  solve [ simpl in *; intuition; eauto; repeat match goal with
+          | |- context[is_val ?e] => do !rewrite is_val_spec
+          end; simplify_val; by tac ].
+Ltac solve_val := solve_val by eauto.
+
+(* Misc *)
+Lemma is_val_of_val v : is_val (of_val v).
+Proof. solve_val. Qed.
+#[export] Hint Resolve is_val_of_val : core.
+
+(* Literals, operators, expressions, and values have decidable equality. *)
+Global Instance base_lit_eq_dec : EqDecision base_lit.
+Proof. solve_decision. Defined.
+Global Instance un_op_eq_dec : EqDecision un_op.
+Proof. solve_decision. Defined.
+Global Instance bin_op_eq_dec : EqDecision bin_op.
+Proof. solve_decision. Defined.
+Global Instance expr_eq_dec : EqDecision expr.
+Proof. solve_decision. Defined.
+Global Instance val_eq_dec : EqDecision val.
+Proof. solve_decision. Defined.
+
+(* Coq prop [is_val] is decidable. *)
+Global Instance is_val_dec e : Decision (is_val e).
+Proof.
+  induction e;
+  repeat match goal with
+  | H: Decision (is_val ?e) |- _ => destruct H
+  end; solve [left; solve_val | right; simpl in *; intuition].
+Defined.
+
+(** Substitution *)
+(** [subst x es e] substitutes the expression [es] for the variable [x] in the
+  * expression [e]. If [x] is a bound variable, it would not be substituted. *)
+Fixpoint subst (x : string) (es : expr) (e : expr) : expr :=
+  match e with
+  | Lit _ => e
+  | Var y => if decide (x = y) then es else e
+  | Lam y e' => if decide (BNamed x = y) then e else Lam y (subst x es e')
+  | App e1 e2 => App (subst x es e1) (subst x es e2)
+  | UnOp op e' => UnOp op (subst x es e')
+  | BinOp op e1 e2 => BinOp op (subst x es e1) (subst x es e2)
+  | If e0 e1 e2 => If (subst x es e0) (subst x es e1) (subst x es e2)
+  | TApp e' => TApp (subst x es e')
+  | TLam e' => TLam (subst x es e')
+  | Pack e' => Pack (subst x es e')
+  | Unpack y e1 e2 =>
+      Unpack y (subst x es e1) (if decide (BNamed x = y) then e2 else subst x es e2)
+  | Pair e1 e2 => Pair (subst x es e1) (subst x es e2)
+  | Fst e' => Fst (subst x es e')
+  | Snd e' => Snd (subst x es e')
+  | InjL e' => InjL (subst x es e')
+  | InjR e' => InjR (subst x es e')
+  | Case e0 e1 e2 =>
+      Case (subst x es e0) (subst x es e1) (subst x es e2)
+  end.
+
+Definition subst' (mx : binder) (es : expr) (e : expr) : expr :=
+  match mx with BNamed x => subst x es e | BAnon => e end.
+
+
+(** The stepping relation *)
+Definition un_op_eval (op : un_op) (l : base_lit) : option base_lit :=
+  match op, l with
+  | NegOp, LitBool b => Some $ LitBool $ negb b
+  | MinusUnOp, LitInt n => Some $ LitInt (-n)
+  | LenOp, LitString s => Some $ LitInt $ Z.of_nat $ String.length s
+  | _, _ => None
+  end.
+
+Definition bin_op_eval (op : bin_op) (l1 l2 : base_lit) : option base_lit :=
+  match op, l1, l2 with
+  | PlusOp, LitInt n1, LitInt n2 =>
+      Some $ LitInt (n1 + n2)
+  | MinusOp, LitInt n1, LitInt n2 =>
+      Some $ LitInt (n1 - n2)
+  | MultOp, LitInt n1, LitInt n2 =>
+      Some $ LitInt (n1 * n2)
+  | LtOp, LitInt n1, LitInt n2 =>
+      Some $ LitBool $ bool_decide (n1 < n2)%Z
+  | LeOp, LitInt n1, LitInt n2 =>
+      Some $ LitBool $ bool_decide (n1 <= n2)%Z
+  | GtOp, LitInt n1, LitInt n2 =>
+      Some $ LitBool $ bool_decide (n1 > n2)%Z
+  | GeOp, LitInt n1, LitInt n2 =>
+      Some $ LitBool $ bool_decide (n1 >= n2)%Z
+  | AndOp, LitBool b1, LitBool b2 =>
+      Some $ LitBool (b1 && b2)
+  | OrOp, LitBool b1, LitBool b2 =>
+      Some $ LitBool (b1 || b2)
+  | SubOp, LitBool b1, LitBool b2 =>
+      Some $ LitBool $ bool_decide (b1 → b2)
+  | ConcatOp, LitString s1, LitString s2 =>
+      Some $ LitString (s1 ++ s2)
+  | PrefixOp, LitString s1, LitString s2 =>
+      Some $ LitBool $ String.prefix s1 s2
+  | SubstrOp, LitString s1, LitString s2 =>
+      Some $ LitBool $
+        match String.index 0 s1 s2 with
+        | Some _ => true
+        | None => false
+        end
+  | EqOp, _, _ =>
+      Some $ LitBool $ bool_decide (l1 = l2)
+  | NeqOp, _, _ =>
+      Some $ LitBool $ bool_decide (l1 ≠ l2)
+  | _, _, _ => None
+  end.
+
+Inductive base_step : expr → expr → Prop :=
+  | BetaS x e1 e2 e' :
+      is_val e2 →
+      e' = subst' x e2 e1 →
+      base_step (App (Lam x e1) e2) e'
+  | TBetaS e :
+      base_step (TApp (TLam e)) e
+  | UnpackS x e1 e2 e' :
+      is_val e1 →
+      e' = subst' x e1 e2 →
+      base_step (Unpack x (Pack e1) e2) e'
+  | UnOpS op l l' :
+      un_op_eval op l = Some l' →
+      base_step (UnOp op $ Lit l) (Lit l')
+  | BinOpS op l1 l2 l' :
+      bin_op_eval op l1 l2 = Some l' →
+      base_step (BinOp op (Lit l1) (Lit l2)) (Lit l')
+  | IfTrueS e1 e2 :
+      base_step (If (Lit $ LitBool true) e1 e2) e1
+  | IfFalseS e1 e2 :
+      base_step (If (Lit $ LitBool false) e1 e2) e2
+  | FstS e1 e2 :
+      is_val e1 →
+      is_val e2 →
+      base_step (Fst (Pair e1 e2)) e1
+  | SndS e1 e2 :
+      is_val e1 →
+      is_val e2 →
+      base_step (Snd (Pair e1 e2)) e2
+  | CaseLS e1 e2 e :
+      is_val e →
+      base_step (Case (InjL e) e1 e2) (App e1 e)
+  | CaseRS e1 e2 e :
+      is_val e →
+      base_step (Case (InjR e) e1 e2) (App e2 e)
+  .
+
+
+(** We define evaluation contexts *)
+Inductive ectx :=
+  | HoleCtx
+  | AppLCtx (K: ectx) (v2 : val)
+  | AppRCtx (e1 : expr) (K: ectx)
+  | TAppCtx (K: ectx)
+  | PackCtx (K: ectx)
+  | UnpackCtx (x : binder) (K: ectx) (e2 : expr)
+  | UnOpCtx (op : un_op) (K: ectx)
+  | BinOpLCtx (op : bin_op) (K: ectx) (v2 : val)
+  | BinOpRCtx (op : bin_op) (e1 : expr) (K: ectx)
+  | IfCtx (K: ectx) (e1 e2 : expr)
+  | PairLCtx (K: ectx) (v2 : val)
+  | PairRCtx (e1 : expr) (K: ectx)
+  | FstCtx (K: ectx)
+  | SndCtx (K: ectx)
+  | InjLCtx (K: ectx)
+  | InjRCtx (K: ectx)
+  | CaseCtx (K: ectx) (e1 : expr) (e2 : expr) .
+
+Fixpoint fill (K : ectx) (e : expr) : expr :=
+  match K with
+  | HoleCtx => e
+  | AppLCtx K v2 => App (fill K e) (of_val v2)
+  | AppRCtx e1 K => App e1 (fill K e)
+  | TAppCtx K => TApp (fill K e)
+  | PackCtx K => Pack (fill K e)
+  | UnpackCtx x K e2 => Unpack x (fill K e) e2
+  | UnOpCtx op K => UnOp op (fill K e)
+  | BinOpLCtx op K v2 => BinOp op (fill K e) (of_val v2)
+  | BinOpRCtx op e1 K => BinOp op e1 (fill K e)
+  | IfCtx K e1 e2 => If (fill K e) e1 e2
+  | PairLCtx K v2 => Pair (fill K e) (of_val v2)
+  | PairRCtx e1 K => Pair e1 (fill K e)
+  | FstCtx K => Fst (fill K e)
+  | SndCtx K => Snd (fill K e)
+  | InjLCtx K => InjL (fill K e)
+  | InjRCtx K => InjR (fill K e)
+  | CaseCtx K e1 e2 => Case (fill K e) e1 e2
+  end.
+
+Fixpoint comp_ectx (K: ectx) (K' : ectx) : ectx :=
+  match K with
+  | HoleCtx => K'
+  | AppLCtx K v2 => AppLCtx (comp_ectx K K') v2
+  | AppRCtx e1 K => AppRCtx e1 (comp_ectx K K')
+  | TAppCtx K => TAppCtx (comp_ectx K K')
+  | PackCtx K => PackCtx (comp_ectx K K')
+  | UnpackCtx x K e2 => UnpackCtx x (comp_ectx K K') e2
+  | UnOpCtx op K => UnOpCtx op (comp_ectx K K')
+  | BinOpLCtx op K v2 => BinOpLCtx op (comp_ectx K K') v2
+  | BinOpRCtx op e1 K => BinOpRCtx op e1 (comp_ectx K K')
+  | IfCtx K e1 e2 => IfCtx (comp_ectx K K') e1 e2
+  | PairLCtx K v2 => PairLCtx (comp_ectx K K') v2
+  | PairRCtx e1 K => PairRCtx e1 (comp_ectx K K')
+  | FstCtx K => FstCtx (comp_ectx K K')
+  | SndCtx K => SndCtx (comp_ectx K K')
+  | InjLCtx K => InjLCtx (comp_ectx K K')
+  | InjRCtx K => InjRCtx (comp_ectx K K')
+  | CaseCtx K e1 e2 => CaseCtx (comp_ectx K K') e1 e2
+  end.
+
+(** Contextual step *)
+Inductive contextual_step (e1 : expr) (e2 : expr) : Prop :=
+  Ectx_step K e1' e2' :
+    e1 = fill K e1' →
+    e2 = fill K e2' →
+    base_step e1' e2' →
+    contextual_step e1 e2.
+Definition reducible (e : expr) := ∃ e', contextual_step e e'.
+
+Definition empty_ectx := HoleCtx.
+
+(** Basic properties about the evaluation contexts. *)
+Lemma fill_empty e : fill empty_ectx e = e.
+Proof. done. Qed.
+
+Lemma fill_comp (K1 K2 : ectx) e : fill K1 (fill K2 e) = fill (comp_ectx K1 K2) e.
+Proof. induction K1; simpl; congruence. Qed.
+
+
+(** Basic properties about the contextual step. *)
+Lemma base_contextual_step e1 e2 :
+  base_step e1 e2 → contextual_step e1 e2.
+Proof. apply Ectx_step with empty_ectx; by rewrite ?fill_empty. Qed.
+
+Lemma fill_contextual_step K e1 e2 :
+  contextual_step e1 e2 → contextual_step (fill K e1) (fill K e2).
+Proof.
+  destruct 1 as [K' e1' e2' -> ->].
+  rewrite !fill_comp. by econstructor.
+Qed.
+
+Lemma fill_rtc_contextual_step K e1 e2 :
+  rtc contextual_step e1 e2 → rtc contextual_step (fill K e1) (fill K e2).
+Proof.
+  induction 1; try naive_solver.
+  etrans; eauto using rtc_once, fill_contextual_step.
+Qed.
+
+
+
+Fixpoint is_closed (X : list string) (e : expr) : bool :=
+   match e with
+  | Var x => bool_decide (x ∈ X)
+  | Lam x e => is_closed (x :b: X) e
+  | Unpack x e1 e2 => is_closed X e1 && is_closed (x :b: X) e2
+  | Lit _ => true
+  | UnOp _ e | Fst e | Snd e | InjL e | InjR e | TApp e | TLam e | Pack e =>
+      is_closed X e
+  | App e1 e2 | BinOp _ e1 e2 | Pair e1 e2 =>
+      is_closed X e1 && is_closed X e2
+  |  If e0 e1 e2 | Case e0 e1 e2 =>
+      is_closed X e0 && is_closed X e1 && is_closed X e2
+  end.
+
+#[export] Instance is_closed_proof_irrel X e : ProofIrrel (is_closed X e).
+Proof. apply _. Defined.
+#[export] Instance is_closed_dec X e : Decision (is_closed X e).
+Proof. apply _. Defined.
+
+(** closed expressions *)
+Lemma is_closed_weaken X Y e : is_closed X e → X ⊆ Y → is_closed Y e.
+Proof. revert X Y; induction e; naive_solver (eauto; set_solver). Qed.
+
+Lemma is_closed_weaken_nil X e : is_closed [] e → is_closed X e.
+Proof. intros. by apply is_closed_weaken with [], list_subseteq_nil. Qed.
+
+Lemma is_closed_subst X e x es :
+  is_closed [] es → is_closed (x :: X) e → is_closed X (subst x es e).
+Proof.
+  intros ?; induction e in X |-*; simpl; intros ?; destruct_and?; split_and?; simplify_option_eq; eauto using is_closed_weaken with set_solver.
+Qed.
+Lemma is_closed_subst' X e x es :
+  is_closed [] es → is_closed (x :b: X) e → is_closed X (subst' x es e).
+Proof. destruct x; eauto using is_closed_subst. Qed.
+
+(** Substitution lemmas *)
+Lemma subst_is_closed X e x es : is_closed X e → x ∉ X → subst x es e = e.
+Proof.
+  induction e in X |-*; simpl; rewrite ?bool_decide_spec, ?andb_True; intros ??;
+    repeat case_decide; simplify_eq; simpl; f_equal; intuition eauto with set_solver.
+Qed.
+
+Lemma subst_is_closed_nil e x es : is_closed [] e → subst x es e = e.
+Proof. intros. apply subst_is_closed with []; set_solver. Qed.
+Lemma subst'_is_closed_nil e x es : is_closed [] e → subst' x es e = e.
+Proof. destruct x as [ | x]; eauto using subst_is_closed_nil. Qed.
